Other Modal Logics Subsets (#196)
* S4 ⊂ Grz

* S5 ⊂ Triv

* Grz ⊂ Triv

* S4Dot2 ⊂ S4Dot3

* S4Dot3 ⊂ S5

* Update about S4.3

Foundation/Modal/Logic/WellKnown.lean
@@ -16,9 +16,11 @@ import Foundation.Modal.Kripke.Hilbert.KT
 import Foundation.Modal.Kripke.Hilbert.KTB
 import Foundation.Modal.Kripke.Hilbert.S4
 import Foundation.Modal.Kripke.Hilbert.S4Dot2
+import Foundation.Modal.Kripke.Hilbert.S4Dot3
 import Foundation.Modal.Kripke.Hilbert.S5
 import Foundation.Modal.Kripke.Hilbert.Triv
 import Foundation.Modal.Kripke.Hilbert.Ver
+import Foundation.Modal.Hilbert.S5Grz
 import Foundation.Modal.Logic.Basic
 import Foundation.Modal.System.KT
 
@@ -102,11 +104,16 @@ lemma S4Dot2.eq_ReflexiveTransitiveConfluentKripkeFrameClass_Logic : Logic.S4Dot
 
 
 protected abbrev S4Dot3 : Logic := Hilbert.S4Dot3.logic
-
+lemma S4Dot3.eq_ReflexiveTransitiveConnectedKripkeFrameClass_Logic : Logic.S4Dot3 = Kripke.ReflexiveTransitiveConnectedFrameClass.logic
+  := eq_Hilbert_Logic_KripkeFrameClass_Logic
 
 protected abbrev S5 : Logic := Hilbert.S5.logic
 lemma S5.eq_ReflexiveEuclideanKripkeFrameClass_Logic : Logic.S5 = Kripke.ReflexiveEuclideanFrameClass.logic
   := eq_Hilbert_Logic_KripkeFrameClass_Logic
+lemma S5.eq_UniversalKripkeFrameClass_Logic : Logic.S5 = Kripke.UniversalFrameClass.logic
+  := eq_Hilbert_Logic_KripkeFrameClass_Logic
+
+protected abbrev S5Grz : Logic := Hilbert.S5Grz.logic
 
 
 protected abbrev GL : Logic := Hilbert.GL.logic
@@ -164,31 +171,6 @@ theorem KTB_ssubset_S5 : Logic.KTB ⊂ Logic.S5 := by
         constructor;
         . omega;
         . use 2;
-          constructor <;> omega;
-
-theorem S4_ssubset_S5 : Logic.S4 ⊂ Logic.S5 := by
-  constructor;
-  . rw [S4.eq_ReflexiveTransitiveKripkeFrameClass_Logic, S5.eq_ReflexiveEuclideanKripkeFrameClass_Logic];
-    rintro φ hφ F ⟨F_refl, F_eucl⟩;
-    apply hφ;
-    refine ⟨F_refl, trans_of_refl_eucl F_refl F_eucl⟩;
-  . suffices ∃ φ, Hilbert.S5 ⊢! φ ∧ ¬ReflexiveTransitiveFrameClass ⊧ φ by simpa [S4.eq_ReflexiveTransitiveKripkeFrameClass_Logic];
-    use Axioms.Five (.atom 0);
-    constructor;
-    . exact axiomFive!;
-    . apply Formula.Kripke.ValidOnFrameClass.not_of_exists_model_world;
-      let M : Model := ⟨⟨Fin 3, λ x y => (x = y) ∨ (x = 0 ∧ y = 1) ∨ (x = 0 ∧ y = 2)⟩, (λ w _ => w = 2)⟩;
-      use M, 0;
-      constructor;
-      . refine ⟨?_, ?_⟩;
-        . tauto;
-        . simp [Transitive];
-          omega;
-      . suffices (0 : M.World) ≺ 2 ∧ ∃ x : M.World, (0 : M.World) ≺ x ∧ ¬x ≺ 2 by
-          simpa [M, Semantics.Realize, Satisfies];
-        constructor;
-        . tauto;
-        . use 1;
           constructor <;> omega;
 
 theorem KD45_ssubset_S5 : Logic.KD45 ⊂ Logic.S5 := by
@@ -729,6 +711,142 @@ theorem S4_ssubset_S4Dot2 : Logic.S4 ⊂ Logic.S4Dot2 := by
           constructor;
           . omega;
           . omega;
+
+theorem S4Dot2_ssubset_S4Dot3 : Logic.S4Dot2 ⊂ Logic.S4Dot3 := by
+  constructor;
+  . rw [S4Dot2.eq_ReflexiveTransitiveConfluentKripkeFrameClass_Logic, S4Dot3.eq_ReflexiveTransitiveConnectedKripkeFrameClass_Logic];
+    rintro φ hφ F ⟨F_refl, F_trans, F_conn⟩;
+    apply hφ;
+    refine ⟨?_, ?_, ?_⟩;
+    . exact F_refl;
+    . exact F_trans;
+    . exact confluent_of_refl_connected F_refl F_conn;
+  . suffices ∃ φ, Hilbert.S4Dot3 ⊢! φ ∧ ¬ReflexiveTransitiveConfluentFrameClass ⊧ φ by
+      simpa [S4Dot2.eq_ReflexiveTransitiveConfluentKripkeFrameClass_Logic];
+    use Axioms.Dot3 (.atom 0) (.atom 1);
+    constructor;
+    . exact axiomDot3!;
+    . apply Formula.Kripke.ValidOnFrameClass.not_of_exists_model_world;
+      let M : Model := ⟨⟨Fin 4, λ x y => ¬(x = 1 ∧ y = 2) ∧ ¬(x = 2 ∧ y = 1) ∧ (x ≤ y)⟩, λ w a => (a = 0 ∧ (w = 1 ∨ w = 3)) ∨ (a = 1 ∧ (w = 2 ∨ w = 3))⟩;
+      use M, 0;
+      constructor;
+      . simp only [Set.mem_setOf_eq];
+        refine ⟨?_, ?_, ?_⟩;
+        . simp [M, Reflexive]; omega;
+        . simp [M, Transitive]; omega;
+        . rintro x y z ⟨Rxy, Ryz⟩;
+          use 3;
+          constructor <;> omega;
+      . apply Kripke.Satisfies.or_def.not.mpr;
+        push_neg;
+        constructor;
+        . apply Kripke.Satisfies.box_def.not.mpr;
+          push_neg;
+          use 1;
+          simp [Satisfies, Semantics.Realize, M];
+          constructor <;> omega;
+        . apply Kripke.Satisfies.box_def.not.mpr;
+          push_neg;
+          use 2;
+          simp [Satisfies, Semantics.Realize, M];
+          constructor <;> omega;
+
+theorem S4Dot3_ssubset_S5 : Logic.S4Dot3 ⊂ Logic.S5 := by
+  constructor;
+  . rw [S4Dot3.eq_ReflexiveTransitiveConnectedKripkeFrameClass_Logic, S5.eq_UniversalKripkeFrameClass_Logic];
+    rintro φ hφ F F_univ;
+    apply hφ;
+    refine ⟨?_, ?_, ?_⟩;
+    . unfold Reflexive; intros; apply F_univ;
+    . unfold Transitive; intros; apply F_univ;
+    . unfold Connected; intros; constructor; apply F_univ;
+  . suffices ∃ φ, Hilbert.S5 ⊢! φ ∧ ¬ReflexiveTransitiveConnectedFrameClass ⊧ φ by
+      simpa [S4Dot3.eq_ReflexiveTransitiveConnectedKripkeFrameClass_Logic];
+    use Axioms.Five (.atom 0);
+    constructor;
+    . exact axiomFive!;
+    . apply Formula.Kripke.ValidOnFrameClass.not_of_exists_model_world;
+      let M : Model := ⟨⟨Fin 2, λ x y => x ≤ y⟩, λ w a => (w = 0)⟩;
+      use M, 0;
+      constructor;
+      . simp only [Set.mem_setOf_eq];
+        refine ⟨?_, ?_, ?_⟩;
+        . simp [M, Reflexive];
+        . simp [M, Transitive]; omega;
+        . rintro x y z ⟨Rxy, Ryz⟩; omega;
+      . suffices (0 : M.World) ≺ 0 ∧ ∃ x, (0 : M.World) ≺ x ∧ ¬x ≺ 0 by
+          simpa [M, Semantics.Realize, Satisfies];
+        constructor;
+        . omega;
+        . use 1;
+          constructor <;> omega;
+
+lemma S4_ssubset_S5 : Logic.S4 ⊂ Logic.S5 := by
+  trans Logic.S4Dot2;
+  . exact S4_ssubset_S4Dot2;
+  . trans Logic.S4Dot3;
+    . exact S4Dot2_ssubset_S4Dot3;
+    . exact S4Dot3_ssubset_S5;
+
+theorem S4_ssubset_Grz : Logic.S4 ⊂ Logic.Grz := by
+  constructor;
+  . exact Hilbert.weakerThan_of_dominate_axioms $ by simp;
+  . suffices ∃ φ, Hilbert.Grz ⊢! φ ∧ ¬ReflexiveTransitiveFrameClass ⊧ φ by simpa [S4.eq_ReflexiveTransitiveKripkeFrameClass_Logic];
+    use Axioms.Grz (.atom 0)
+    constructor;
+    . exact axiomGrz!;
+    . apply Formula.Kripke.ValidOnFrameClass.not_of_exists_model_world;
+      use ⟨⟨Fin 2, λ x y => True⟩, λ w _ => w = 1⟩, 0;
+      simp [Reflexive, Transitive, Semantics.Realize, Satisfies];
+
+lemma S5Grz_eq_Triv : Logic.S5Grz = Logic.Triv := by
+  ext φ;
+  exact Hilbert.iff_provable_S5Grz_provable_Triv;
+
+lemma S5_ssubset_S5Grz : Logic.S5 ⊂ Logic.S5Grz := by
+  constructor;
+  . exact Hilbert.weakerThan_of_dominate_axioms $ by simp;
+  . suffices ∃ φ, Hilbert.S5Grz ⊢! φ ∧ ¬UniversalFrameClass ⊧ φ by simpa [S5.eq_UniversalKripkeFrameClass_Logic];
+    use Axioms.Grz (.atom 0)
+    constructor;
+    . exact axiomGrz!;
+    . apply Formula.Kripke.ValidOnFrameClass.not_of_exists_model_world;
+      use ⟨⟨Fin 2, λ x y => True⟩, λ w _ => w = 1⟩, 0;
+      simp [Universal, Semantics.Realize, Satisfies];
+
+theorem S5_ssubset_Triv : Logic.S5 ⊂ Logic.Triv := by
+  convert S5_ssubset_S5Grz;
+  exact S5Grz_eq_Triv.symm;
+
+-- TODO: more refactor for operating finite frame
+lemma Grz_ssubset_S5Grz : Logic.Grz ⊂ Logic.S5Grz := by
+  constructor;
+  . exact Hilbert.weakerThan_of_dominate_axioms $ by simp;
+  . suffices ∃ φ, Hilbert.S5Grz ⊢! φ ∧ ¬ReflexiveTransitiveAntiSymmetricFiniteFrameClass ⊧ φ by simpa [Grz.eq_ReflexiveTransitiveAntiSymmetricFiniteKripkeFrameClass_Logic];
+    use Axioms.Five (.atom 0)
+    constructor;
+    . exact axiomFive!;
+    . apply Formula.Kripke.ValidOnFrameClass.not_of_exists_frame;
+      let F : FiniteFrame := ⟨Fin 2, λ x y => x ≤ y⟩;
+      use F.toFrame;
+      constructor;
+      . use F;
+        refine ⟨⟨?_, ?_, ?_⟩, rfl⟩;
+        . simp [F, Reflexive];
+        . simp [F, Transitive]; omega;
+        . simp [F, AntiSymmetric]; omega;
+      . apply ValidOnFrame.not_of_exists_valuation_world;
+        use (λ w _ => w = 0), 0;
+        suffices (0 : F.World) ≺ 0 ∧ ∃ x, (0 : F.World) ≺ x ∧ ¬x ≺ 0 by
+          simpa [Semantics.Realize, Satisfies, ValidOnFrame];
+        constructor;
+        . omega;
+        . use 1;
+          constructor <;> omega;
+
+theorem Grz_ssubset_Triv : Logic.Grz ⊂ Logic.Triv := by
+  convert Grz_ssubset_S5Grz;
+  exact S5Grz_eq_Triv.symm;
 
 end Logic
 
